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1 The Trivial Inequality

The trivial inequality states that

x2 ≥ 0, x ∈ R

which is quite straightforward.

2 The AM-GM Inequality

The AM-GM inequality is very commonly used in inequality problems. First make sure you are familiar with the
definitions of Arithmetic Means and Geometric Means. It states that if a1, a2, ..., an are positive reals,

a1 + a2 + ...+ an
n

≥ (a1a2...an)1/n

and equality holds if and only if ai are all equal (i = 1, 2, ..., n).
Proof. This is an inductive proof. For n = 1 it is obvious. For n = 2,

a1 + a2
2

≥
√
a1a2 (1)

⇔ a21 + 2a1a2 + a22
4

≥ a1a2

⇔ a21 − 2a1a2 + a22 ≥ 0

⇔ (a1 − a2)2 ≥ 0

which is true.
Now we claim that the statement is true for all n = 2k where k is any positive integer.
Assume the statement is true for n = 2k−1. Then,

a1 + a2 + ...+ an
n

≥ (a1a2...an)1/n

Because (1) is true,

a1+a2+...+an
n + an+1+an+2+...+a2n

n

2
≥

√
a1 + a2 + ...+ an

n

an+1 + an+2 + ...+ a2n
n

≥
√

(a1a2...an)1/n(an+1an+2...a2n)1/n

=
√

(a1a2...a2n)1/n

= (a1a2...a2n)1/(2n)

and thus 2n = 2k is true as well. So by induction this claim is proven.
Now we work backwards to prove for n is not a power of two. Assume our statement is true for n, then

a1 + a2 + ...+ an
n

≥ (a1a2...an)1/n
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Let an = a1+a2+...+an−1

n−1 ,

a1 + a2 + ...+ an−1 + a1+a2+...+an−1

n−1

n
≥ (a1a2...an−1

a1 + a2 + ...+ an−1

n− 1
)1/n

n(a1+a2+...+an−1)
n−1

n
≥ (a1a2...an−1

a1 + a2 + ...+ an−1

n− 1
)1/n

(
a1 + a2 + ...+ an−1

n− 1
)n ≥ a1a2...an−1

a1 + a2 + ...+ an−1

n− 1

(
a1 + a2 + ...+ an−1

n− 1
)n−1 ≥ a1a2...an−1

a1 + a2 + ...+ an−1

n− 1
≥ (a1a2...an−1)1/(n−1)

and therefore we have proved that the statement is true even if n is not a power of two. In conclusion we have proved
that the statement is true for all n ∈ N. (Q.E.D)

3 The Cauchy-Schwarz Inequality

The formal definition of Cauchy-Schwarz is in the form of vectors. However, we can also write it in a more understandable
way: If a1, a2, ..., an and b1, b2, ..., bn are all real numbers,

(a21 + a22 + ...+ a2n)(b21 + b22 + ...+ b2n) ≥ (a1b1 + a2b2 + ...anbn)2

and equality holds if and only if ai
bi

are all equal (i = 1, 2, ..., n).
The proof can be done by simple induction, so it is left as an exercise for the reader. We hereby present another proof:
Proof. Consider the polynomial:

P (x) = (a1x+ b1)2 + (a2x+ b2)2 + ...+ (anx+ bn)2

= (a21 + a22 + ...+ a2n)x2 + 2(a1b1 + a2b2 + ...+ anbn)x+ (b21 + b22 + ...+ b2n)

Since P (x) ≥ 0 and P (x) is a quadratic equation, therefore ∆ = B2 − 4AC ≤ 0.

4(a1b1 + ...+ anbn)2 − 4(a21 + ...+ a2n)(b21 + ...+ b2n) ≤ 0

and the result follows. (Q.E.D)

4 The Rearrangement Inequality

Let’s consider a real-life example: You have the opportunity to receive notes of RM100, RM20 and RM5 such that the
number of notes is 8, 5, 2 (any order of this). How would you take to get the maximum amount of money? How about
the minimum?
Do you get the idea now? This is precisely the rearrangement inequality, which, in formal definitions, is: If (a1, a2, ...an)
and (b1, b2, ...bn) are both increasing sequences,

a1b1 + a2b2 + ...+ anbn

≥ a1bσ1
+ a2bσ2

+ ...+ anbσn

≥ a1bn + a2bn−1 + ...+ anb1

where (σ1, σ2, ..., σn) is any permutation of (1, 2, ..., n).

5 IMO shortlist problem

Let a, b, c be positive reals and abc = 1. Prove that

1

a3(b+ c)
+

1

b3(a+ c)
+

1

c3(a+ b)
≥ 3

2

Solution 1.
Let the original equation be A. Then

A =
b2c2

a(b+ c)
+

a2c2

b(a+ c)
+

a2b2

c(a+ b)
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(a(b+ c) + b(c+ a) + c(a+ b))·A ≥ (
√
a(b+ c)

bc√
a(b+ c)

+
√
b(c+ a)

ca√
b(c+ a)

+
√
c(a+ b)

ab√
c(a+ b)

)2

= (bc+ ca+ ab)2

≥ (bc+ ca+ ab)· 3(bc· ca· ab)1/3

= 3(bc+ ca+ ab)

i.e. 2(bc+ ca+ ab).A ≥ 3(bc+ ca+ ab) and the conclusion follows. (Q.E.D)

Solution 2.
By Titu’s Lemma,

x21
y1

+
x22
y2

+ ...+
x2n
yn
≥ (x1 + x2 + ...+ xn)2

y1 + y2 + ...+ yn

Now

A =
b2c2

a(b+ c)
+

a2c2

b(a+ c)
+

a2b2

c(a+ b)

≥ (bc+ ca+ ab)2

2(bc+ ca+ ab)

=
1

2
(bc+ ca+ ab)

≥ 1

2
(3(bc· ca· ab)1/3)

=
3

2

(Q.E.D)

Solution 3.
From the AM-GM inequality,

a2 + b2 ≥ 2ab

a2

b
≥ 2a− b

Now

A =
1

4
(

4b2c2

a(b+ c)
+

4a2c2

b(a+ c)
+

4a2b2

c(a+ b)
)

≥ 1

4
(4bc− (ab+ ac) + 4ca− (ab+ bc) + 4ab− (ac+ bc))

=
1

2
(bc+ ca+ ab)

≥ 1

2
(3(bc· ca· ab)1/3)

=
3

2

(Q.E.D)

6 Real Problems

Assume in all of these problems, the unknowns are all positive reals.

1. Prove the extended form of the AM-GM inequality, which is the QM-AM-GM-HM inequality:√
a21 + ...+ a2n

n
≥ a1 + ...+ an

n
≥ (a1...an)1/n ≥ n

1
a1

+ ...+ 1
an

(You just need to prove the left and right hand side.)

2. If 3a+ b = 1, what is the minimum value of a2 + b2? (2017/HuaLuoGeng)

3. Prove that a2 + b2 + c2 ≥ ab+ bc+ ca.

4. If a+ b+ c = 6, what is the maximum value of a3b2c? (2017/ChenJingRun)

5. If a+ b ≤ 1, what is the minimum value of ab+ 1
ab? (BIMO Junior Test 2018)
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